Started adding Lets (very broken)

01Source/SourceLanguage.thy
@@ -5,19 +5,19 @@ begin
 section \<open>Source Language\<close>
 
 text \<open>We now define our source language. It consists of the untyped lambda calculus, enhanced with 
-numbers and arithmetic. There are two main challenges with implementing the untyped lambda calculus: 
-the non-termination of evaluation, and capture-avoiding substitution. We cannot address the first 
-here, since our language as it stands does in fact admit unnormalizable terms like
-\<open>App\<^sub>s (Lam\<^sub>s x (App\<^sub>s (Var\<^sub>s x) (Var\<^sub>s x))) (Lam\<^sub>s x (App\<^sub>s (Var\<^sub>s x) (Var\<^sub>s x)))\<close>; after typechecking, we will 
-lower our sights to the simply-typed subset of our language and be able to prove normalization then.
-As for substitution, for now we take the brute-force approach of renaming every binder to a fresh 
-variable every time we substitute past it. We will shortly switch to a nameless Debruijn-index 
-representation to make substitution simpler, but we want to keep our source language as close to an 
-intuitive, "human-readable" version as possible. After all, changing this sort of behaviour to one 
-more easily implemented on a computer is the essence of compilation.\<close>
+let-expressions and uninterpreted numbers. There are two main challenges with implementing the 
+untyped lambda calculus: the non-termination of evaluation, and capture-avoiding substitution. We 
+cannot address the first here, since our language as it stands does in fact admit unnormalizable 
+terms like \<open>App\<^sub>s (Lam\<^sub>s x (App\<^sub>s (Var\<^sub>s x) (Var\<^sub>s x))) (Lam\<^sub>s x (App\<^sub>s (Var\<^sub>s x) (Var\<^sub>s x)))\<close>; after 
+typechecking, we will lower our sights to the simply-typed subset of our language and be able to 
+prove normalization then. As for substitution, for now we take the brute-force approach of renaming 
+every binder to a fresh variable every time we substitute past it. We will shortly switch to a 
+nameless Debruijn-index representation to make substitution simpler, but we want to keep our source 
+language as close to an intuitive, "human-readable" version as possible. After all, changing this 
+sort of behaviour to one more easily implemented on a computer is the essence of compilation.\<close>
 
-text \<open>Our concrete datatype is parameterized on an annotation on each binder; this will enable us to
-reuse the same datatype for the typed version.\<close>
+text \<open>Our concrete datatype is parameterized on an annotation on each lambda binder; this will 
+enable us to reuse the same datatype for the typed version.\<close>
 
 (* TODO: products and sums *)
 
@@ -26,6 +26,7 @@ datatype 'a expr\<^sub>s =
   | Const\<^sub>s nat
   | Lam\<^sub>s var 'a "'a expr\<^sub>s"
   | App\<^sub>s "'a expr\<^sub>s" "'a expr\<^sub>s"
+  | Let\<^sub>s var "'a expr\<^sub>s" "'a expr\<^sub>s"
 
 text \<open>Only numbers and lambda-abstractions are values:\<close>
 
@@ -34,6 +35,7 @@ primrec value\<^sub>s :: "'a expr\<^sub>s \<Rightarrow> bool" where
 | "value\<^sub>s (Const\<^sub>s n) = True" 
 | "value\<^sub>s (Lam\<^sub>s x t e) = True" 
 | "value\<^sub>s (App\<^sub>s e\<^sub>1 e\<^sub>2) = False" 
+| "value\<^sub>s (Let\<^sub>s x e\<^sub>1 e\<^sub>2) = False" 
 
 text \<open>We define free and bound variables in the usual way:\<close>
 
@@ -42,12 +44,14 @@ primrec free_vars\<^sub>s :: "'a expr\<^sub>s \<Rightarrow> var set" where
 | "free_vars\<^sub>s (Const\<^sub>s n) = {}"
 | "free_vars\<^sub>s (Lam\<^sub>s x t e) = free_vars\<^sub>s e - {x}"
 | "free_vars\<^sub>s (App\<^sub>s e\<^sub>1 e\<^sub>2) = free_vars\<^sub>s e\<^sub>1 \<union> free_vars\<^sub>s e\<^sub>2"
+| "free_vars\<^sub>s (Let\<^sub>s x e\<^sub>1 e\<^sub>2) = free_vars\<^sub>s e\<^sub>1 \<union> (free_vars\<^sub>s e\<^sub>2 - {x})"
 
 primrec bound_vars\<^sub>s :: "'a expr\<^sub>s \<Rightarrow> var set" where
   "bound_vars\<^sub>s (Var\<^sub>s x) = {}"
 | "bound_vars\<^sub>s (Const\<^sub>s n) = {}"
 | "bound_vars\<^sub>s (Lam\<^sub>s x t e) = insert x (bound_vars\<^sub>s e)"
 | "bound_vars\<^sub>s (App\<^sub>s e\<^sub>1 e\<^sub>2) = bound_vars\<^sub>s e\<^sub>1 \<union> bound_vars\<^sub>s e\<^sub>2"
+| "bound_vars\<^sub>s (Let\<^sub>s x e\<^sub>1 e\<^sub>2) = insert x (bound_vars\<^sub>s e\<^sub>1 \<union> bound_vars\<^sub>s e\<^sub>2)"
 
 definition all_vars\<^sub>s :: "'a expr\<^sub>s \<Rightarrow> var set" where
   "all_vars\<^sub>s e \<equiv> free_vars\<^sub>s e \<union> bound_vars\<^sub>s e"
@@ -67,6 +71,9 @@ lemma all_vars_lam [simp]: "all_vars\<^sub>s (Lam\<^sub>s x t e) = insert x (all
 lemma all_vars_app [simp]: "all_vars\<^sub>s (App\<^sub>s e\<^sub>1 e\<^sub>2) = all_vars\<^sub>s e\<^sub>1 \<union> all_vars\<^sub>s e\<^sub>2"
   by (auto simp add: all_vars\<^sub>s_def)
 
+lemma all_vars_let [simp]: "all_vars\<^sub>s (Let\<^sub>s x e\<^sub>1 e\<^sub>2) = insert x (all_vars\<^sub>s e\<^sub>1 \<union> all_vars\<^sub>s e\<^sub>2)"
+  by (auto simp add: all_vars\<^sub>s_def)
+
 text \<open>Next, we define a limited form of substitution that simply swaps one variable for another. 
 Note that this function is unsafe if the replacement variable is bound in the expression; we will 
 only ever use it in \<open>subst\<^sub>s\<close>, where we generate a fresh variable for it.\<close>
@@ -76,6 +83,8 @@ primrec subst_var\<^sub>s :: "var \<Rightarrow> var \<Rightarrow> 'a expr\<^sub>
 | "subst_var\<^sub>s x x' (Const\<^sub>s n) = Const\<^sub>s n"
 | "subst_var\<^sub>s x x' (Lam\<^sub>s y t e) = Lam\<^sub>s y t (if x = y then e else subst_var\<^sub>s x x' e)"
 | "subst_var\<^sub>s x x' (App\<^sub>s e\<^sub>1 e\<^sub>2) = App\<^sub>s (subst_var\<^sub>s x x' e\<^sub>1) (subst_var\<^sub>s x x' e\<^sub>2)"
+| "subst_var\<^sub>s x x' (Let\<^sub>s y e\<^sub>1 e\<^sub>2) = 
+    Let\<^sub>s y (subst_var\<^sub>s x x' e\<^sub>1) (if x = y then e\<^sub>2 else subst_var\<^sub>s x x' e\<^sub>2)"
 
 lemma size_subst_var [simp]: "size (subst_var\<^sub>s x x' e) = size e"
   by (induction e) simp_all
@@ -98,6 +107,9 @@ fun subst\<^sub>s :: "var \<Rightarrow> 'a expr\<^sub>s \<Rightarrow> 'a expr\<^
     let z = fresh (all_vars\<^sub>s e' \<union> all_vars\<^sub>s e \<union> {x, y})
     in Lam\<^sub>s z t (subst\<^sub>s x e' (subst_var\<^sub>s y z e)))"
 | "subst\<^sub>s x e' (App\<^sub>s e\<^sub>1 e\<^sub>2) = App\<^sub>s (subst\<^sub>s x e' e\<^sub>1) (subst\<^sub>s x e' e\<^sub>2)"
+| "subst\<^sub>s x e' (Let\<^sub>s y e\<^sub>1 e\<^sub>2) = (
+    let z = fresh (all_vars\<^sub>s e' \<union> all_vars\<^sub>s e\<^sub>2 \<union> {x, y})
+    in Let\<^sub>s z (subst\<^sub>s x e' e\<^sub>1) (subst\<^sub>s x e' (subst_var\<^sub>s y z e\<^sub>2)))"
 
 lemma free_vars_subst_var [simp]: "free_vars\<^sub>s e \<subseteq> insert x xs \<Longrightarrow> 
  free_vars\<^sub>s (subst_var\<^sub>s x x' e) \<subseteq> insert x' xs"
@@ -106,6 +118,11 @@ proof (induction e arbitrary: xs)
   hence "free_vars\<^sub>s e \<subseteq> insert x (insert y xs)" by auto
   with Lam\<^sub>s have "free_vars\<^sub>s (subst_var\<^sub>s x x' e) \<subseteq> insert x' (insert y xs)" by simp
   with Lam\<^sub>s show ?case by auto
+next
+  case (Let\<^sub>s y e\<^sub>1 e\<^sub>2)
+  hence "free_vars\<^sub>s e\<^sub>2 \<subseteq> insert x (insert y xs)" by auto
+  with Let\<^sub>s have "free_vars\<^sub>s (subst_var\<^sub>s x x' e\<^sub>2) \<subseteq> insert x' (insert y xs)" by simp
+  with Let\<^sub>s show ?case by auto
 qed auto
 
 lemma free_vars_subst [simp]: "free_vars\<^sub>s e \<subseteq> insert x xs \<Longrightarrow> free_vars\<^sub>s e' \<subseteq> xs \<Longrightarrow> 
@@ -117,6 +134,15 @@ proof (induction x e' e arbitrary: xs rule: subst\<^sub>s.induct)
   hence "free_vars\<^sub>s (subst_var\<^sub>s y ?z e) \<subseteq> insert ?z (insert x xs)" by simp
   hence "free_vars\<^sub>s (subst_var\<^sub>s y ?z e) \<subseteq> insert x (insert ?z xs)" by auto
   with 3 show ?case by (auto simp add: Let_def)
+next
+  case (5 x e' y e\<^sub>1 e\<^sub>2)
+  let ?z = "fresh (all_vars\<^sub>s e' \<union> all_vars\<^sub>s e\<^sub>2 \<union> {x, y})"
+  from 5 have "free_vars\<^sub>s e\<^sub>2 \<subseteq> insert y (insert x xs)" by auto
+  hence "free_vars\<^sub>s (subst_var\<^sub>s y ?z e\<^sub>2) \<subseteq> insert ?z (insert x xs)" by simp
+  hence X: "free_vars\<^sub>s (subst_var\<^sub>s y ?z e\<^sub>2) \<subseteq> insert x (insert ?z xs)" by auto
+  from 5 have "free_vars\<^sub>s e' \<subseteq> insert ?z xs" by auto
+  with 5 X have "free_vars\<^sub>s (subst\<^sub>s x e' (subst_var\<^sub>s y ?z e\<^sub>2)) \<subseteq> insert ?z xs" by auto
+  with 5 show ?case by (auto simp add: Let_def)
 qed auto
 
 text \<open>Now, we define big-step applicative-order evaluation. It is represented by an inductive 
@@ -128,6 +154,7 @@ inductive eval\<^sub>s :: "'a expr\<^sub>s \<Rightarrow> 'a expr\<^sub>s \<Right
   ev\<^sub>s_const [simp]: "Const\<^sub>s n \<Down>\<^sub>s Const\<^sub>s n"
 | ev\<^sub>s_lam [simp]: "Lam\<^sub>s x t e \<Down>\<^sub>s Lam\<^sub>s x t e"
 | ev\<^sub>s_app [simp]: "e\<^sub>1 \<Down>\<^sub>s Lam\<^sub>s x t e\<^sub>1' \<Longrightarrow> e\<^sub>2 \<Down>\<^sub>s v\<^sub>2 \<Longrightarrow> subst\<^sub>s x v\<^sub>2 e\<^sub>1' \<Down>\<^sub>s v \<Longrightarrow> App\<^sub>s e\<^sub>1 e\<^sub>2 \<Down>\<^sub>s v"
+| ev\<^sub>s_let [simp]: "e\<^sub>1 \<Down>\<^sub>s v\<^sub>1 \<Longrightarrow> subst\<^sub>s x v\<^sub>1 e\<^sub>2 \<Down>\<^sub>s v\<^sub>2 \<Longrightarrow> Let\<^sub>s x e\<^sub>1 e\<^sub>2 \<Down>\<^sub>s v\<^sub>2"
 
 lemma free_vars_eval [simp]: "e \<Down>\<^sub>s v \<Longrightarrow> free_vars\<^sub>s e = {} \<Longrightarrow> free_vars\<^sub>s v = {}"
 proof (induction e v rule: eval\<^sub>s.induct)
@@ -135,6 +162,11 @@ proof (induction e v rule: eval\<^sub>s.induct)
   hence "free_vars\<^sub>s e\<^sub>1' \<subseteq> insert x {} \<and> free_vars\<^sub>s v\<^sub>2 \<subseteq> {}" by simp
   hence "free_vars\<^sub>s (subst\<^sub>s x v\<^sub>2 e\<^sub>1') \<subseteq> {}" by (metis free_vars_subst)
   with ev\<^sub>s_app show ?case by simp
+next
+  case (ev\<^sub>s_let e\<^sub>1 v\<^sub>1 x e\<^sub>2 v\<^sub>2)
+  hence "free_vars\<^sub>s e\<^sub>2 \<subseteq> insert x {} \<and> free_vars\<^sub>s v\<^sub>1 \<subseteq> {}" by simp
+  hence "free_vars\<^sub>s (subst\<^sub>s x v\<^sub>1 e\<^sub>2) \<subseteq> {}" by (metis free_vars_subst)
+  with ev\<^sub>s_let show ?case by simp
 qed simp_all
 
 lemma eval_to_value [simp]: "e \<Down>\<^sub>s v \<Longrightarrow> value\<^sub>s v"
@@ -156,16 +188,20 @@ next
 next
   case (ev\<^sub>s_app e\<^sub>1 x e\<^sub>1' e\<^sub>2 v\<^sub>2 v)
   from ev\<^sub>s_app(7, 1, 2, 3, 4, 5, 6) show ?case by (induction rule: eval\<^sub>s.cases) blast+
+next
+  case (ev\<^sub>s_let e\<^sub>1 v\<^sub>1 x e\<^sub>2 v\<^sub>2 t)
+  from ev\<^sub>s_let(5, 1, 2, 3, 4) show ?case by (induction rule: eval\<^sub>s.cases) blast+
 qed
 
 text \<open>We also define a no-shadowing predicate on our expressions, where no variable is ever bound 
-twice in the same scope.\<close>
+twice in the same scope. This will be useful when we later remove names from the representation.\<close>
 
 primrec no_shadowing\<^sub>s :: "'a expr\<^sub>s \<Rightarrow> bool" where
   "no_shadowing\<^sub>s (Var\<^sub>s x) = True"
 | "no_shadowing\<^sub>s (Const\<^sub>s n) = True"
 | "no_shadowing\<^sub>s (Lam\<^sub>s x t e) = (no_shadowing\<^sub>s e \<and> x \<notin> bound_vars\<^sub>s e)"
 | "no_shadowing\<^sub>s (App\<^sub>s e\<^sub>1 e\<^sub>2) = (no_shadowing\<^sub>s e\<^sub>1 \<and> no_shadowing\<^sub>s e\<^sub>2)"
+| "no_shadowing\<^sub>s (Let\<^sub>s x e\<^sub>1 e\<^sub>2) = (no_shadowing\<^sub>s e\<^sub>1 \<and> no_shadowing\<^sub>s e\<^sub>2 \<and> x \<notin> bound_vars\<^sub>s e\<^sub>2)"
 
 lemma now_shadowing_subst_var [simp]: "no_shadowing\<^sub>s (subst_var\<^sub>s x y e) = no_shadowing\<^sub>s e"
   by (induction e) simp_all
@@ -181,6 +217,10 @@ primrec remove_shadows\<^sub>s' :: "var set \<Rightarrow> 'a expr\<^sub>s \<Righ
     in let y = fresh (vs \<union> all_vars\<^sub>s e')
     in Lam\<^sub>s y t (subst_var\<^sub>s x y e'))"
 | "remove_shadows\<^sub>s' vs (App\<^sub>s e\<^sub>1 e\<^sub>2) = App\<^sub>s (remove_shadows\<^sub>s' vs e\<^sub>1) (remove_shadows\<^sub>s' vs e\<^sub>2)"
+| "remove_shadows\<^sub>s' vs (Let\<^sub>s x e\<^sub>1 e\<^sub>2) = (
+    let e\<^sub>2' = remove_shadows\<^sub>s' (insert x vs) e\<^sub>2
+    in let y = fresh (vs \<union> all_vars\<^sub>s e\<^sub>2')
+    in Let\<^sub>s y (remove_shadows\<^sub>s' vs e\<^sub>1) (subst_var\<^sub>s x y e\<^sub>2'))"
 
 definition remove_shadows\<^sub>s :: "'a expr\<^sub>s \<Rightarrow> 'a expr\<^sub>s" where
   "remove_shadows\<^sub>s e \<equiv> remove_shadows\<^sub>s' {} e"
@@ -193,6 +233,13 @@ proof (induction e arbitrary: vs)
   from Lam\<^sub>s have "finite (vs \<union> all_vars\<^sub>s ?e)" by simp
   hence "?x \<notin> vs \<union> all_vars\<^sub>s ?e" by (metis fresh_is_fresh)
   with Lam\<^sub>s show ?case by (simp add: Let_def all_vars\<^sub>s_def)
+next
+  case (Let\<^sub>s x e\<^sub>1 e\<^sub>2)
+  let ?e\<^sub>2 = "remove_shadows\<^sub>s' (insert x vs) e\<^sub>2"
+  let ?x = "fresh (vs \<union> all_vars\<^sub>s ?e\<^sub>2)"
+  from Let\<^sub>s have "finite (vs \<union> all_vars\<^sub>s ?e\<^sub>2)" by simp
+  hence "?x \<notin> vs \<union> all_vars\<^sub>s ?e\<^sub>2" by (metis fresh_is_fresh)
+  with Let\<^sub>s show ?case by (simp add: Let_def all_vars\<^sub>s_def)
 qed simp_all
 
 lemma remove_shadows_no_shadow [simp]: "no_shadowing\<^sub>s (remove_shadows\<^sub>s e)"
@@ -207,6 +254,13 @@ proof (induction e arbitrary: vs)
   from Lam\<^sub>s have "finite (vs \<union> all_vars\<^sub>s ?e)" by simp
   hence "?x \<notin> vs \<union> all_vars\<^sub>s ?e" by (metis fresh_is_fresh)
   with Lam\<^sub>s show ?case by (simp add: Let_def all_vars\<^sub>s_def)
+next
+  case (Let\<^sub>s x e\<^sub>1 e\<^sub>2)
+  let ?e\<^sub>2 = "remove_shadows\<^sub>s' (insert x vs) e\<^sub>2"
+  let ?x = "fresh (vs \<union> all_vars\<^sub>s ?e\<^sub>2)"
+  from Let\<^sub>s have "finite (vs \<union> all_vars\<^sub>s ?e\<^sub>2)" by simp
+  hence "?x \<notin> vs \<union> all_vars\<^sub>s ?e\<^sub>2" by (metis fresh_is_fresh)
+  with Let\<^sub>s show ?case by (simp add: Let_def all_vars\<^sub>s_def)
 qed simp_all
 
 end
